a.
$\frac{1}{n}$
b., c.
$$
\begin{aligned}
T(n)&=\sum_{q=1}^{n}{X_q}(T(q-1)+T(n-q)+\Theta(n)),\\
T(0)&=T(1)=0.\\
\mathbf E[T(n)]&= \mathbf E[\sum_{q=1}^{n}{X_q}(T(q-1)+T(n-q)+\Theta(n))]\\
&= \mathbf E[\sum_{q=1}^{n}{X_q}(T(q-1)+T(n-q))+\Theta(n)]\\
&= \mathbf E[\sum_{q=1}^{n}{X_q}(T(q-1)+T(n-q))]+\Theta(n)\\
&=\sum_{q=1}^{n}\mathbf E[{X_q}(T(q-1)+T(n-q))]+\Theta(n)\\
&=\sum_{q=1}^{n}(\mathbf E[X_q]\mathbf E[T(q-1)]+\mathbf E[X_q]\mathbf E[T(n-q)])+\Theta(n)\\
&=\sum_{q=1}^{n}(\frac{1}{n}\mathbf E[T(q-1)]+\frac{1}{n}\mathbf E[T(n-q)])+\Theta(n)\\
&=\frac{1}{n}\sum_{q=1}^{n}(\mathbf E[T(q-1)]+\mathbf E[T(n-q)])+\Theta(n)\\
&=\frac{2}{n}\sum_{q=1}^{n-1}\mathbf E[T(q)]+\Theta(n).
\end{aligned}
$$
d.
$$
\begin{aligned}
\sum_{k=1}^{n-1}k\log{k}&\leq\int_2^n\frac{1}{2}x^2\log{x}-\frac{\ln{2}}{4}x^2
\\&=\frac{1}{2}n^2\log{n}-\frac{\ln{2}}{4}n^2-(2-\ln2)\\
&\leq \frac{1}{2}n^2\log{n}-\frac{1}{8}n^2
\end{aligned}
$$
e.
Assume the inequality that for some $a$, $\mathbf E[T(k)] \le ak\log{k}$ true for $2\le k\le n-1$,then
$$
\begin{aligned}
\mathbf E[T(n)]&=\frac{2}{n}\sum_{q=1}^{n-1}\mathbf E[T(q)]+\Theta(n)\\
&\le \frac{2}{n}\sum_{q=1}^{n-1}aq\log q+\Theta(n)\\
&\le \frac{2a}{n}(\frac{1}{2}n^2\log{n}-\frac{1}{8}n^2)+\Theta(n)\\
&=an\log{n}-\frac{a}{4}n+\Theta(n),
\end{aligned}
$$
there exist $a$ large enough so that
$$
\mathbf E[T(n)]\le an\log{n}.
$$
Base case stands:
$$
T(2)=\frac{2}{n}T(1)+\Theta(2)=\Theta(2),\\
T(2)\le an\log{n}\quad \text{for }a \text{ large enough}.
$$
Therefore $\mathbf E[T(n)]=\text{O}(n\log{n})$.
